parse32 vldata size

examples/lowparse/LowParse.SLow.VLData.fst
@@ -7,11 +7,11 @@ module Seq = FStar.Seq
 module U8 = FStar.UInt8
 module U16 = FStar.UInt16
 module U32 = FStar.UInt32
-module E = FStar.Kremlin.Endianness
+module E = LowParse.BigEndian
 module Cast = FStar.Int.Cast
 module B32 = FStar.Bytes
 
-#reset-options "--z3cliopt smt.arith.nl=false --z3rlimit 64 --max_ifuel 64 --max_fuel 64"
+#reset-options "--z3cliopt smt.arith.nl=false --z3rlimit 128 --max_ifuel 64 --max_fuel 64"
 
 let pow2_8 () : Lemma (pow2 8 == 256) [SMTPat (pow2 8)] = assert_norm (pow2 8 == 256)
 let pow2_16 () : Lemma (pow2 16 == 65536) [SMTPat (pow2 16)] = assert_norm (pow2 16 == 65536)
@@ -216,6 +216,159 @@ let serialize32_bounded_integer
   | 3 -> serialize_bounded_integer_conv 3 sz serialize32_bounded_integer_3
   | 4 -> serialize_bounded_integer_conv 4 sz serialize32_bounded_integer_4
 
+#reset-options "--z3rlimit 32"
+
+inline_for_extraction
+let decode32_bounded_integer_1
+ (b: B32.lbytes 1)
+: Tot (y: bounded_integer 1 { y == decode_bounded_integer 1 (B32.reveal b) } )
+= let r = B32.get b 0ul in
+  assert (r == B32.index b 0);
+  B32.index_reveal b 0;
+  E.be_to_n_1_spec (B32.reveal b);
+  let res : U32.t = Cast.uint8_to_uint32 r in
+  assert (res == (decode_bounded_integer 1 (B32.reveal b) <: U32.t));
+  assert (U32.v res < pow2 (FStar.Mul.op_Star 8 1));
+  let (res: bounded_integer 1) = res in
+  (res <: (y: bounded_integer 1 { y == decode_bounded_integer 1 (B32.reveal b) }))
+
+inline_for_extraction
+let parse32_bounded_integer_1 : parser32 (parse_bounded_integer 1) =
+  decode_bounded_integer_injective 1;
+  make_total_constant_size_parser32 1 1ul
+    (decode_bounded_integer 1)
+    ()
+    (decode32_bounded_integer_1)
+
+let synth_bounded_integer_2
+  (x: U16.t)
+: GTot (bounded_integer 2)
+= Cast.uint16_to_uint32 x
+
+let synth_bounded_integer_2_inj
+  ()
+: Lemma
+  (forall (x x' : U16.t) . synth_bounded_integer_2 x == synth_bounded_integer_2 x' ==> x == x')
+= ()
+
+#reset-options "--z3rlimit 256 --max_fuel 64 --max_ifuel 64"
+
+let parse_bounded_integer_2_spec
+  ()
+: Lemma
+  (forall (input: bytes) . parse (parse_bounded_integer 2) input == parse (parse_u16 `parse_synth` synth_bounded_integer_2) input)
+= let f
+    (input: bytes { Seq.length input == 2 })
+  : Lemma
+    ((decode_u16 `compose` synth_bounded_integer_2) input == decode_bounded_integer 2 input)
+  = E.be_to_n_2_spec input;
+    E.lemma_be_to_n_is_bounded input;
+    assert (U16.v (decode_u16 input) == U32.v (decode_bounded_integer 2 input));
+    assert (U32.v ((decode_u16 `compose` synth_bounded_integer_2) input) == U32.v (decode_bounded_integer 2 input));
+    U32.v_inj ((decode_u16 `compose` synth_bounded_integer_2) input) (decode_bounded_integer 2 input)
+  in
+  Classical.forall_intro f;
+  decode_u16_injective ();
+  synth_bounded_integer_2_inj ();
+  make_total_constant_size_parser_compose 2 U16.t (bounded_integer 2) (decode_u16) (synth_bounded_integer_2);
+  assert_norm (forall (input: bytes) . parse (parse_bounded_integer 2) input == parse (make_total_constant_size_parser 2 (bounded_integer 2) (decode_u16 `compose` synth_bounded_integer_2)) input)
+
+inline_for_extraction
+let parse32_bounded_integer_2 : parser32 (parse_bounded_integer 2) =
+  fun (input: bytes32) -> (
+    let res = parse32_synth parse_u16 synth_bounded_integer_2 (fun (x: U16.t) -> (Cast.uint16_to_uint32 x <: (y: bounded_integer 2 { y == synth_bounded_integer_2 x } ))) parse32_u16 () input in
+    parse_bounded_integer_2_spec ();
+    (res <: (res: option (bounded_integer 2 * U32.t) { parser32_correct (parse_bounded_integer 2) input res} ))
+  )
+
+(*
+inline_for_extraction
+let decode32_bounded_integer_2
+ (b: B32.lbytes 2)
+: Tot (y: bounded_integer 2 { y == decode_bounded_integer 2 (B32.reveal b) } )
+= let b0r = B32.get b 0ul in
+  assert (b0r == B32.index b 0);
+  B32.index_reveal b 0;
+  let b0 = Cast.uint8_to_uint32 b0r in
+  let b1r = B32.get b 1ul in
+  assert (b1r == B32.index b 1);
+  B32.index_reveal b 1;
+  let b1 = Cast.uint8_to_uint32 b1r in
+  let res = U32.add b1 (U32.mul 256ul b0) in
+  E.be_to_n_2_spec (B32.reveal b);
+  E.lemma_be_to_n_is_bounded (B32.reveal b);
+  assert (res == (decode_bounded_integer 2 (B32.reveal b) <: U32.t));
+  assert (U32.v res < pow2 (FStar.Mul.op_Star 8 2));
+  let (res: bounded_integer 2) = res in
+  (res <: (y: bounded_integer 2 { y == decode_bounded_integer 2 (B32.reveal b) }))
+
+inline_for_extraction
+let parse32_bounded_integer_2 : parser32 (parse_bounded_integer 2) =
+  decode_bounded_integer_injective 2;
+  make_total_constant_size_parser32 2 2ul
+    (decode_bounded_integer 2)
+    ()
+    (decode32_bounded_integer_2)
+*)
+
+#reset-options "--z3rlimit 1024 --z3refresh  --smtencoding.elim_box true --smtencoding.l_arith_repr native --smtencoding.nl_arith_repr wrapped --max_fuel 64 --max_ifuel 64"
+
+inline_for_extraction
+let decode32_bounded_integer_3
+ (b: B32.lbytes 3)
+: Tot (y: bounded_integer 3 { y == decode_bounded_integer 3 (B32.reveal b) } )
+= let b0r = B32.get b 0ul in
+  assert (b0r == B32.index b 0);
+  B32.index_reveal b 0;
+  let b0 = Cast.uint8_to_uint32 b0r in
+  let b1r = B32.get b 1ul in
+  assert (b1r == B32.index b 1);
+  B32.index_reveal b 1;
+  let b1 = Cast.uint8_to_uint32 b1r in
+  let b2r = B32.get b 2ul in
+  assert (b2r == B32.index b 2);
+  B32.index_reveal b 2;
+  let b2 = Cast.uint8_to_uint32 b2r in
+  let res = U32.add b2 (U32.mul 256ul (U32.add b1 (U32.mul 256ul b0))) in
+  E.be_to_n_3_spec (B32.reveal b);
+  E.lemma_be_to_n_is_bounded (B32.reveal b);
+  assert (U32.v res == U32.v (decode_bounded_integer 3 (B32.reveal b) <: U32.t));
+  U32.v_inj res (decode_bounded_integer 3 (B32.reveal b) <: U32.t);
+  assert (U32.v res < pow2 (FStar.Mul.op_Star 8 3));
+  let (res: bounded_integer 3) = res in
+  (res <: (y: bounded_integer 3 { y == decode_bounded_integer 3 (B32.reveal b) }))
+
+#reset-options "--z3rlimit 256 --max_fuel 64 --max_ifuel 64"
+
+inline_for_extraction
+let parse32_bounded_integer_3 : parser32 (parse_bounded_integer 3) =
+  decode_bounded_integer_injective 3;
+  make_total_constant_size_parser32 3 3ul
+    (decode_bounded_integer 3)
+    ()
+    (decode32_bounded_integer_3)
+
+let synth_bounded_integer_4
+  (x: U32.t)
+: GTot (bounded_integer 4)
+= x
+
+let parse_bounded_integer_4_spec
+  ()
+: Lemma
+  (forall (input: bytes) . parse (parse_bounded_integer 4) input == parse (parse_u32 `parse_synth` synth_bounded_integer_4) input)
+= assert (forall (input: bytes { Seq.length input == 4 }) . (decode_u32 `compose` synth_bounded_integer_4) input == decode_bounded_integer 4 input);
+  decode_u32_injective ();
+  make_total_constant_size_parser_compose 4 U32.t (bounded_integer 4) (decode_u32) (synth_bounded_integer_4);
+  assert_norm (forall (input: bytes) . parse (parse_bounded_integer 4) input == parse (make_total_constant_size_parser 4 (bounded_integer 4) (decode_u32 `compose` synth_bounded_integer_4)) input)
+
+inline_for_extraction
+let parse32_bounded_integer_4 : parser32 (parse_bounded_integer 4) =
+  fun (input: bytes32) -> (
+    let res = parse32_synth parse_u32 synth_bounded_integer_4 (fun (x: U32.t) -> (x <: (y: bounded_integer 4 { y == synth_bounded_integer_4 x } ))) parse32_u32 () input in
+    parse_bounded_integer_4_spec ();
+    (res <: (res: option (bounded_integer 4 * U32.t) { parser32_correct (parse_bounded_integer 4) input res} ))
+  )
 
 (* Parsers and serializers for the payload *)
 
